src/program_proof/single/try_decide_proof.v
@@ -1,0 +1,97 @@
+From iris.algebra Require Import gmap lib.mono_nat.
+From iris.proofmode Require Import base tactics classes.
+From iris.bi.lib Require Import fractional.
+From Perennial.program_proof Require Import proof_prelude.
+From Goose.github_com.mit_pdos.gokv.paxi Require Import single.
+From Perennial.program_proof.single Require Import single_proof replica_proof.
+
+Section try_decide_proof.
+
+Context `{!heapG Σ}.
+Context `{paxosG Σ u64}.
+
+Context `{f:nat}.
+
+Lemma wp_Clerk__Prepare ck pid γ reply_ptr dummy_rep (pn:u64) :
+  (* is_Clerk r pid γ -∗ *)
+  {{{
+       own_PrepareReply reply_ptr dummy_rep
+  }}}
+    Clerk__Prepare #ck #pn #reply_ptr
+  {{{
+       reply, RET #();
+            own_PrepareReply reply_ptr reply ∗
+            (⌜reply.(Prep_Success) = false⌝ ∨
+             pn_ptsto f γ (int.nat reply.(Prep_Pn)) (reply.(Prep_Val)) ∗
+             (∀ pn', ⌜pn' < int.nat pn⌝ → ⌜int.nat reply.(Prep_Pn) < pn'⌝ → rejected γ pid pn')
+             )
+  }}}.
+Proof.
+Admitted.
+
+Lemma wp_Clerk__Propose ck pid γ (pn:u64) (val:u64) :
+  (* is_Clerk r pid γ -∗ *)
+  {{{
+       pn_ptsto f γ (int.nat pn) val
+  }}}
+    Clerk__Propose #ck #pn #val
+  {{{
+       (ret:bool), RET #ret;
+       ⌜ret = false⌝ ∨ accepted γ pid (int.nat pn)
+  }}}.
+Proof.
+Admitted.
+
+
+Lemma wp_TryDecide s pid γ (v:u64) (outv_ptr:loc) :
+  is_Replica s pid γ (f:=f) -∗
+  {{{
+       True
+  }}}
+    Replica__TryDecide #s #v #outv_ptr
+  {{{
+        RET #(); True
+  }}}.
+Proof.
+  iIntros "#His !#" (Φ) "Hpre HΦ".
+  wp_lam.
+  wp_pures.
+  iNamed "His".
+  wp_loadField.
+  wp_apply (acquire_spec with "Hmu_inv").
+  iIntros "[Hlocked Hown]".
+  wp_pures.
+  iNamed "Hown".
+  wp_loadField.
+  wp_loadField.
+  wp_apply (release_spec with "[-HΦ]").
+  {
+    iFrame "Hmu_inv Hlocked".
+    iNext.
+    iExists _, _, _, _.
+    iFrame "∗#".
+  }
+  wp_pures.
+
+  wp_apply (typed_mem.wp_AllocAt uint64T).
+  { naive_solver. }
+  iIntros (numPrepared) "HnumPrepared".
+  wp_pures.
+  wp_store.
+
+  wp_apply (typed_mem.wp_AllocAt uint64T).
+  { naive_solver. }
+  iIntros (highestPN) "HhighestPN".
+  wp_pures.
+  wp_store.
+
+  wp_apply (typed_mem.wp_AllocAt uint64T).
+  { naive_solver. }
+  iIntros (highestVal) "HhighestVal".
+  wp_pures.
+  wp_store.
+
+  wp_apply (wp_new_free_lock).
+  iIntros (l) "Hl".
+  wp_pures.
+  (* Need to have read-only ownership of clerks for peers *)
